Isabelle2/R3_Refines_R1.thy
@@ -30,21 +30,53 @@ lemmas amp_defs = ioa_defs ampr1_ioa_def ampr3_ioa_def ghost_ioa_def
 definition inv1 where "inv1 s \<equiv> let r3_s = fst s; h = snd s in
   \<forall> a v . (Packet a (Fwd v)) \<in> network r3_s \<longrightarrow> v \<in> h"
 declare inv1_def[inv_proofs_defs]
-  
+
 lemma inv1:"invariant ghost_ioa inv1"
   apply (rule invariantI)
    apply (simp add:inv1_def amp_defs)
+  apply (rm_reachable)
   apply (simp add:ghost_ioa_def)
-  apply(simp only: split_paired_all)
-  apply (rule IOA.add_hist_trans)
-  
+  apply (simp only: split_paired_all)
+  apply (frule IOA.add_hist_trans(1), drule IOA.add_hist_trans(2))
+  apply (simp add:is_trans_def ampr3_ioa_def ioa_def)
+  apply (drule trans_cases)
+          apply (auto simp add:inv1_def)
+         defer 
+         apply(simp add:receive_2b_def Let_def split:if_splits option.splits)
+        apply(simp add:try_acquire_leadership_def Let_def send_all_def split:if_splits option.splits)
+       apply (metis amp_r3.msg.distinct(13) amp_r3.packet.inject empty_iff receive_1a_def singletonD snd_conv)
+      apply(simp add:receive_2a_def Let_def send_all_def split:if_splits option.splits)
+     apply(simp add:receive_2b_def Let_def send_all_def split:if_splits option.splits)
+    apply(simp add:receive_1b_def receive_1b.msgs_def msgs_def Let_def send_all_def split:if_splits option.splits)
+  subgoal proof -
+    fix a :: "('a, 'v) global_state" and b :: "'v set" and ac :: 'a and bb :: nat and vs :: "nat \<Rightarrow>f ('v \<times> nat) option" and ad :: "('a, 'v) local_state" and bc :: "('a, 'v) packet set" and ae :: 'a and v :: 'v
+    assume a1: "(\<exists>x. finfun_dom (receive_1b.new_log (the (local_state.onebs (local_states a ac) $ bb)) (acceptors (local_states a ac)) (log (local_states a ac))) $ x \<and> (Fwd v::('a, 'v) msg) = (case the_elem (receive_1b.max_per_inst (the (local_state.onebs (local_states a ac) $ bb)) (acceptors (local_states a ac)) $ x) of (v, b) \<Rightarrow> Phase2a x b v)) \<and> ae \<in> acceptors (local_states a ac) \<and> ae \<noteq> local_state.id (local_states a ac)"
+    have "\<And>n p v. (case p of (v, na) \<Rightarrow> Phase2a n na v) \<noteq> (Fwd v::('a, 'v) msg)"
+      by (metis amp_r3.msg.distinct(17) case_prod_conv surj_pair)
+    then show "v \<in> b"
+      using a1 by metis
+  qed
+   apply(simp add: do_2a_def receive_fwd_def Let_def send_all_def split:if_splits option.splits)
+  apply(simp add: do_2a_def propose_def Let_def send_all_def split:if_splits option.splits)
+  done
 
-definition ref_map where "ref_map s \<equiv> \<lparr>
-  ampr1_state.propCmd = propCmd s,
-  ampr1_state.ballot = ballot s,
-  ampr1_state.vote = (\<lambda> i a . vote s $ a $ i),
-  ampr1_state.suggestion = suggestion s,
-  ampr1_state.onebs = onebs s,
-  ampr1_state.leader = ampr2_state.leader s\<rparr>"
+text {*
+TODO: what about letting the ghost state be exactly the state of r1?
+That would give a very simple refinement map, but we will need to prove invariants
+relating the normal state to the ghost state.
+*}
+
+definition ref_map where "ref_map s \<equiv> let r3_s = fst s; ghost_s = snd s in \<lparr>
+  ampr1_state.propCmd = ghost_s,
+  ampr1_state.ballot = (\<lambda> a . local_state.ballot (local_states r3_s a)),
+  ampr1_state.vote = undefined,
+  ampr1_state.suggestion = undefined,
+  ampr1_state.onebs = undefined,
+  ampr1_state.leader = undefined\<rparr>"
+  
+lemma "is_ref_map ref_map ghost_ioa ampr1_ioa" 
+oops
+  
+end
 
 end
